
\begin{problem}
  $l$，$m$，$n$は整数で，$lmn\neq0$のとき
$\displaystyle\int_0^{2x}\cos lx\cos mx\cos nxdx$の値を求めよ．
\end{problem}

\begin{align*}
  &\dumyeq \cos lx  \cos mx  \cos nx \\
  &= \frac12 \left\{ \cos (l+m)x + \cos(l-m)x \right\}\cos nx\\
  &= \frac14
  \left\{ \cos (l+m+x)x + \cos (l+m-n)x + \cos (l-m+n)x + \cos (l-m-n)x \right\}
\end{align*}
より，
\begin{enumerate}[(i)]
  \item $l+m-n = 0$のとき，\\
  $\cos lx  \cos mx  \cos nx = \frac14 \left\{ \cos 2(l+m)x + \cos 2lx + \cos (-2m)x + 1 \right\}$
  であるから，
  \begin{align*}
    &\dumyeq \dint{0}{2\pi} \cos lx \cos mx \cos nx \,dx \\
    &= \frac14 \dint{0}{2\pi}
    \left\{ \cos 2(l+m)x + \cos 2lx + \cos(-2m)x + 1 \right\}\,dx \\
    &= \frac14 \teisekibun{\frac{1}{2(l+m)} \sin 2(l+m)x + \frac{1}{2l} \sin 2lx - \frac{1}{2m}\sin (-2m)x + x}{0}{2\pi} \\
    &= \frac{\pi}2
  \end{align*}

  \item $l-m+n = 0$のとき，\\
  $\cos lx \cos mx \cos nx = \frac14 \left\{ \cos 2(l+n)x + \cos 2lx + \cos(-2n)x + 1 \right\}$
  であるから，
  \begin{align*}
    &\dumyeq \dint{0}{2\pi} \cos lx \cos mx \cos nx \, dx \\
    &= \frac14 \dint{0}{2\pi} \left\{ \cos 2(l+n)x + \cos 2lx + \cos (-2n)x + 1 \right\}\, dx \\
    &= \frac14 \teisekibun{\frac{1}{2(l+n)} \sin 2(l+n)x + \frac{1}{2l}\sin 2lx - \frac{1}{2n} \sin (-2n)x + x}{0}{2\pi}\\
    &= \frac{\pi}2
  \end{align*}

  \item $l-m-n = 0$のとき，\\
  $\cos lx \cos mx \cos nx = \cos 2lx + \cos 2mx + \cos 2nx + 1$
  であるから，
  \begin{align*}
    &\dumyeq \dint{0}{2\pi} \cos lx \cos mx \cos nx \, dx \\
    &= \frac14\dint{0}{2\pi}
    \left\{ \cos 2lx + \cos 2mx + \cos 2nx + 1 \right\} \\
    &= \frac14 \teisekibun{\frac{1}{2l} \sin 2lx + \frac{1}{2m} \sin 2mx + \frac{1}{2n} \sin 2nx + x}{0}{2\pi} \\
    &= \frac{\pi}2
  \end{align*}

  \item $l+m+n = 0$のとき，\\
  $\cos lx \cos mx \cos nx = \cos (-2n)x + \cos(-2n)x + \cos(2l)x + 1$
  であるから，
  \begin{align*}
    &\dumyeq \dint{0}{2\pi} \cos lx \cos mx \cos nx \, dx \\
    &= \frac14 \dint{0}{2\pi}
    \left\{ \cos (-2n)x + \cos(-2n)x + \cos(2l)x + 1 \right\} \\
    &= \frac14 \teisekibun{\frac{1}{-2n}\cos(-2n)x + \frac{1}{-2m}\sin(-2m)x + \frac{1}{2l} \sin (2l)x + x}{0}{2\pi} \\
    &= \frac{\pi}{2}
  \end{align*}

  \item $l+m+n, l+m-n, l-m+n, l-m-n \neq 0$のとき，
  \begin{align*}
    \dumyeq& \dint{0}{2\pi} \cos lx \cos mx \cos nx \, dx \\
    &= \frac14 \left\{ \cos (l+m+x)x + \cos (l+m-n)x + \cos (l-m+n)x + \cos (l-m-n)x \right\} \\
    &= 0
  \end{align*}
\end{enumerate}

(i)～(v)より，

\hfill
$\dint{0}{2\pi} \cos lx\cos mx\cos nx\,dx
= \begin{emcases}
\frac\pi2 &(l+m+n = 0 または l+m-n=0または\\
& l-m+n = 0 まあたは l-m-n = 0 のとき)\\
0 &(l+m+n \neq 0 かつ l+m-n \neq 0 かつ \\
& l-m+n \neq 0 かつ l-m-n \neq 0)
\end{emcases}$
